compiler/proof_vec/equiv_gimli.ec
@@ -16,7 +16,7 @@ proof.
  by proc;auto => &m1 &m2 /> ??; apply (rol32_xor x{m2} bits{m2}). 
 qed. 
 
-equiv Gimli_ref_ref1 : Gimli_ref.M.gimli_body ~ Gimli_ref1.M.gimli_body : ={state} ==> ={res}.
+equiv Gimli_ref_ref1_body : Gimli_ref.M.gimli_body ~ Gimli_ref1.M.gimli_body : ={state} ==> ={res}.
 proof.
   proc.
   while (={round, state});last by auto.
@@ -24,7 +24,16 @@ proof.
   sim; do 2! (call rotate_ref_ref1; sim />).
 qed.
 
-equiv ref1_vec1 : Gimli_ref1.M.gimli_body ~ Gimliv1.M.gimli_body1 : 
+equiv Gimli_ref_ref1 : Gimli_ref.M.gimli ~ Gimli_ref1.M.gimli : 
+   ={istate, Glob.mem } ==> ={Glob.mem}.
+proof.
+  proc.
+  sim 4 4.
+  call Gimli_ref_ref1_body; conseq />.
+  sim.
+qed.
+
+equiv ref1_vec1_body : Gimli_ref1.M.gimli_body ~ Gimliv1.M.gimli_body1 : 
    pack_4u32 (state.[0], state.[1], state.[2] , state.[3] ){1} = x{2} /\
    pack_4u32 (state.[4], state.[5], state.[6] , state.[7] ){1} = y{2} /\
    pack_4u32 (state.[8], state.[9], state.[10], state.[11]){1} = z{2} 
@@ -40,49 +49,49 @@ proof.
   cbv delta => 4!<- _ _; cbv delta => />.
 qed.
 
+equiv ref1_vec1 : Gimli_ref1.M.gimli ~ Gimliv1.M.gimli1 : 
+   istate{1} = state{2} /\ ={Glob.mem} ==> ={Glob.mem}.
+proof.
+  proc.
+  seq 3 3 : 
+   (pack_4u32 (state.[0], state.[1], state.[2] , state.[3] ){1} = x{2} /\
+    pack_4u32 (state.[4], state.[5], state.[6] , state.[7] ){1} = y{2} /\
+    pack_4u32 (state.[8], state.[9], state.[10], state.[11]){1} = z{2}).
+  + unroll for{1} 3.
+    wp; skip => /> &2. admit. (* stuff on memory *)
+  seq 1 1: 
+   (pack_4u32 (state.[0], state.[1], state.[2] , state.[3] ){1} = x{2} /\
+    pack_4u32 (state.[4], state.[5], state.[6] , state.[7] ){1} = y{2} /\
+    pack_4u32 (state.[8], state.[9], state.[10], state.[11]){1} = z{2}).
+  + by call ref1_vec1_body; skip.
+  unroll for{1} 2.
+  wp; skip => /> &2. admit. (* stuff on memory *)
+qed.
+
 axiom rotate24E w :
     x86_VPSHUFB_128  w (W128.of_uint 16028905388486802350658220295983399425)
   = x86_VPSLL_4u32 w (W8.of_uint 24) `^` x86_VPSRL_4u32 w (W8.of_uint 8).
 
 hint simplify rotate24E.
 
-equiv vec1_vec : Gimliv1.M.gimli_body1 ~ Gimliv.M.gimli_body : 
-   ={x,y,z} ==> ={res}.
+equiv vec1_vec : Gimliv1.M.gimli1 ~ Gimliv.M.gimli : 
+   ={state, Glob.mem} ==> ={Glob.mem}.
 proof.
   proc. sim (_:true).
   proc => /=; inline *;wp;skip => />.
 qed.
 
-equiv ref_vec : Gimli_ref.M.gimli_body ~ Gimliv.M.gimli_body : 
-   pack_4u32 (state.[0], state.[1], state.[2] , state.[3] ){1} = x{2} /\
-   pack_4u32 (state.[4], state.[5], state.[6] , state.[7] ){1} = y{2} /\
-   pack_4u32 (state.[8], state.[9], state.[10], state.[11]){1} = z{2} 
-   ==>
-   pack_4u32 (res.[0], res.[1], res.[2] , res.[3] ){1} = res.`1{2} /\
-   pack_4u32 (res.[4], res.[5], res.[6] , res.[7] ){1} = res.`2{2} /\
-   pack_4u32 (res.[8], res.[9], res.[10], res.[11]){1} = res.`3{2}.
-proof.
-  transitivity Gimli_ref1.M.gimli_body 
-    (={state} ==> ={res})
-    (pack_4u32 (state.[0], state.[1], state.[2] , state.[3] ){1} = x{2} /\
-   pack_4u32 (state.[4], state.[5], state.[6] , state.[7] ){1} = y{2} /\
-   pack_4u32 (state.[8], state.[9], state.[10], state.[11]){1} = z{2} 
-   ==>
-   pack_4u32 (res.[0], res.[1], res.[2] , res.[3] ){1} = res.`1{2} /\
-   pack_4u32 (res.[4], res.[5], res.[6] , res.[7] ){1} = res.`2{2} /\
-   pack_4u32 (res.[8], res.[9], res.[10], res.[11]){1} = res.`3{2}) => //.
-  + by move=> &m1 &m2 [#]???; exists state{m1}.  
-  by apply Gimli_ref_ref1.
-  transitivity Gimliv1.M.gimli_body1
-   (pack_4u32 (state.[0], state.[1], state.[2] , state.[3] ){1} = x{2} /\
-   pack_4u32 (state.[4], state.[5], state.[6] , state.[7] ){1} = y{2} /\
-   pack_4u32 (state.[8], state.[9], state.[10], state.[11]){1} = z{2} 
-   ==>
-   pack_4u32 (res.[0], res.[1], res.[2] , res.[3] ){1} = res.`1{2} /\
-   pack_4u32 (res.[4], res.[5], res.[6] , res.[7] ){1} = res.`2{2} /\
-   pack_4u32 (res.[8], res.[9], res.[10], res.[11]){1} = res.`3{2})
-   (={x,y,z} ==> ={res}) => //.
-  + by move=> &m1 &m2 [#]???; exists (x,y,z){m2}.
+equiv ref_vec : Gimli_ref.M.gimli ~ Gimliv.M.gimli : 
+  istate{1} = state{2} /\ ={Glob.mem} ==> ={Glob.mem}.
+  transitivity Gimli_ref1.M.gimli
+    (={istate, Glob.mem} ==> ={Glob.mem})
+    (istate{1} = state{2} /\ ={Glob.mem} ==> ={Glob.mem}) => //.
+  + by move=> &1 &2 />; exists Glob.mem{2} state{2}.  
+  + by apply Gimli_ref_ref1.
+  transitivity Gimliv1.M.gimli1
+    (istate{1} = state{2} /\ ={Glob.mem} ==> ={Glob.mem}) 
+    (={state,Glob.mem} ==> ={Glob.mem}) => //.
+  + by move=> &1 &2 />; exists Glob.mem{2} state{2}.  
   + by apply ref1_vec1.
   by apply vec1_vec.   
 qed.
