compiler/proof_vec/gimliv_ct_proof.ec
@@ -1,6 +1,8 @@
 require import Jasmin_model Gimliv_ct.
 
-equiv gimli_body_ct : M.gimli_body ~ M.gimli_body : ={M.leakages} ==> ={M.leakages}.
+(* [state] is a pointer allowing to initialize the state of gimli *)
+(* Since it is an address, its value is leak, and should be public *)
+equiv gimli_ct : M.gimli ~ M.gimli : ={state, M.leakages} ==> ={M.leakages}.
 proof.
   proc; inline *; sim.
 qed.
