compiler/proof_vec/gimliv_safe_proof.ec
@@ -8,3 +8,28 @@ proof.
   inline *; wp; skip; rewrite /is_init => />.
 qed.
 
+(* TODO move this *)
+axiom addw0 (w : W64.t) : w + W64.zeros = w.
+axiom of_uint0 : W64.of_uint 0 = W64.zeros.
+
+axiom is_valid_store128 mem sz ptr1 ptr2 w : 
+  is_valid (storeW128 mem ptr2 w) ptr1 sz = is_valid mem ptr1 sz.
+hint simplify is_valid_store128.
+
+hoare gimliS : M.gimli : 
+  M.safe /\
+  is_valid Glob.mem state W128 /\
+  is_valid Glob.mem (state + W64.of_uint 16) W128 /\
+  is_valid Glob.mem (state + W64.of_uint 32) W128
+  ==> 
+  M.safe.
+proof.
+  proc.
+  wp; call gimli_bodyS; wp; skip.
+  cbv delta => /> &1.  
+  rewrite of_uint0 addw0 => />.
+qed.
+
+
+
+
